end of day 30/12/18

michael_formal/Contexts.thy
@@ -238,7 +238,8 @@ definition satisfies_context :: "datastate \<Rightarrow> context \<Rightarrow> b
 
 (* Does t2 subsume t1? *)
 definition subsumes :: "context \<Rightarrow> transition \<Rightarrow> transition \<Rightarrow> bool" where (* Corresponds to Algorithm 2 in Foster et. al. *)
-  "subsumes c t2 t1 \<equiv> (\<forall>r i. (cval (medial c (Guard t1) r) i = Some True) \<longrightarrow> (cval (medial c (Guard t2) r) i) = Some True) \<and>
+  "subsumes c t2 t1 \<equiv> Label t1 = Label t2 \<and> Arity t1 = Arity t2 \<and> length (Outputs t1) = length (Outputs t2) \<and>
+                      (\<forall>r i. (cval (medial c (Guard t1) r) i = Some True) \<longrightarrow> (cval (medial c (Guard t2) r) i) = Some True) \<and>
                       (\<forall> i r. satisfies_context r c \<longrightarrow> apply_guards (Guard t1) (join_ir i r) \<longrightarrow> apply_outputs (Outputs t1) (join_ir i r) = apply_outputs (Outputs t2) (join_ir i r)) \<and>
                       (\<forall>r i. cval (posterior (medial c (Guard t1)) t2 r) i = Some True \<longrightarrow> (cval (posterior c t1 r) i = Some True) \<or> (posterior c t1 r) = Undef) \<and>
                       (consistent (posterior c t1) \<longrightarrow> consistent (posterior c t2))"
